implement arrays with pointers

ulib/experimental/Steel.Array.fst
@@ -1,5 +1,5 @@
 (*
-   Copyright 2020 Microsoft Research
+   Copyright 2021 Microsoft Research
 
    Licensed under the Apache License, Version 2.0 (the "License");
    you may not use this file except in compliance with the License.
@@ -16,26 +16,272 @@
 
 module Steel.Array
 
-open Steel.Effect.Atomic
-open Steel.Reference
+module P = Steel.Pointer
 
-let array t = ref (Seq.seq t)
+noeq
+type array t = {
+  from: P.t t;
+  to: Ghost.erased size_t;
+  free_perm: perm;
+  prf: squash (
+    if P.g_is_null from
+    then size_v to == 0 /\ free_perm == full_perm // for unicity
+    else size_v (P.offset from) + size_v to <= size_v (P.base_array_len (P.base from)));
+}
 
-let is_array r = ptr r
-let array_sel r = ptr_sel r
+let len a = Ghost.reveal a.to
+
+let null (a: Type) : Tot (array a) = {
+  from = P.null a;
+  to = zero_size;
+  free_perm = full_perm;
+  prf = ();
+}
+
+let g_is_null a = P.g_is_null a.from
+
+let range_of_array
+  (#t: Type)
+  (a: array t)
+  (p: perm)
+: Tot P.range
+= {
+  P.range_from = 0;
+  P.range_to = size_v a.to;
+  P.range_write_perm = p;
+  P.range_free_perm = a.free_perm;
+  P.range_prf = ();
+}
+
+let varray0 (#t: Type) (a: array t) (p: perm) : Tot vprop =
+  P.vptr_range a.from (range_of_array a p)
+
+let is_array r p = hp_of (varray0 r p)
+
+let array_sel r p = fun h -> sel_of (varray0 r p) h
+
+let intro_varrayp
+  (#opened: _)
+  (#t: Type)
+  (ptr: P.t t)
+  (rg: P.range)
+  (a: array t)
+  (p: perm)
+: SteelGhost unit opened
+    (P.vptr_range ptr rg)
+    (fun _ -> varrayp a p)
+    (fun _ ->
+      ptr == a.from /\
+      rg == range_of_array a p
+    )
+    (fun h _ h' -> (h' (varrayp a p) <: Seq.seq t) == h (P.vptr_range ptr rg))
+=
+  change_slprop_rel
+    (P.vptr_range ptr rg)
+    (varrayp a p)
+    (fun x y -> x == y)
+    (fun _ -> ())
+
+let elim_varrayp
+  (#opened: _)
+  (#t: Type)
+  (a: array t)
+  (p: perm)
+: SteelGhost unit opened
+    (varrayp a p)
+    (fun _ -> P.vptr_range a.from (range_of_array a p))
+    (fun _ -> True)
+    (fun h _ h' ->
+      (h' (P.vptr_range a.from (range_of_array a p)) <: Seq.seq t) == h (varrayp a p)
+    )
+=
+  change_slprop_rel
+    (varrayp a p)
+    (P.vptr_range a.from (range_of_array a p))
+    (fun x y -> x == y)
+    (fun _ -> ())
+
+let varrayp_not_null a p =
+  elim_varrayp a p;
+  P.vptr_range_not_null a.from _;
+  intro_varrayp a.from _ a p
+
+let is_null x r =
+  change_slprop_rel
+    (varrayp_or_null x r)
+    (P.vptr_range_or_null x.from (range_of_array x r))
+    (fun u v -> u == v)
+    (fun _ -> ());
+  let res = P.is_null x.from _ in
+  change_slprop_rel
+    (P.vptr_range_or_null x.from (range_of_array x r))
+    (varrayp_or_null x r)
+    (fun u v -> u == v)
+    (fun _ -> ());
+  return res
+
+let adjacent r1 r2 =
+  P.g_is_null r1.from == P.g_is_null r2.from /\
+  begin if P.g_is_null r1.from
+  then True
+  else
+    P.base r1.from == P.base r2.from /\
+    size_v (P.offset r1.from) + size_v r1.to == size_v (P.offset r2.from)
+  end
+
+let merge r1 r2 = {
+  from = r1.from;
+  to = r1.to `size_add` r2.to;
+  free_perm = if g_is_null r1 then r1.free_perm else r1.free_perm `sum_perm` r2.free_perm;
+  prf = ();
+}
+
+let merge_assoc r1 r2 r3 = ()
+
+let gsplit r i =
+  if g_is_null r
+  then (r, r)
+  else
+  let rl = {
+    from = r.from;
+    to = i;
+    free_perm = half_perm r.free_perm;
+    prf = ();
+  } in
+  let rr = {
+    from = P.g_add r.from i;
+    to = r.to `size_sub` i;
+    free_perm = half_perm r.free_perm;
+    prf = ();
+  } in
+  (rl, rr)
+
+#set-options "--ide_id_info_off"
+
+let splitp a p i =
+  elim_varrayp a _;
+  let pr_from = P.add a.from _ i in
+  let _ = P.move a.from pr_from _ in
+  let tmp = P.split pr_from _ in
+  let _ = P.move pr_from a.from (P.GPair?.fst _) in
+  let res = ({
+    from = a.from;
+    to = i;
+    free_perm = half_perm a.free_perm;
+    prf = ();
+  }, {
+    from = pr_from;
+    to = a.to `size_sub` i;
+    free_perm = half_perm a.free_perm;
+    prf = ();
+  }) in
+  intro_varrayp a.from _ (fst res) p;
+  intro_varrayp pr_from _ (snd res) p;
+  return res
+
+let joinp al ar p =
+  elim_varrayp al _;
+  elim_varrayp ar _;
+  let _ = P.merge_left al.from ar.from _ _ in
+  let res = {
+    from = al.from;
+    to = al.to `size_add` ar.to;
+    free_perm = al.free_perm `sum_perm` ar.free_perm;
+    prf = ();
+  } in
+  intro_varrayp al.from _ res p;
+  return res
+
+let freeable a =
+  P.g_is_null a.from == false /\
+  P.base_array_freeable (P.base a.from) /\
+  size_v (P.offset a.from) == 0 /\
+  Ghost.reveal a.to == P.base_array_len (P.base a.from) /\
+  a.free_perm == full_perm
+
+val intro_varrayp_or_null
+  (#opened: _)
+  (#t: Type)
+  (ptr: P.t t)
+  (rg: P.range)
+  (a: array t)
+  (p: perm)
+: SteelGhost unit opened
+    (P.vptr_range_or_null ptr rg)
+    (fun _ -> varrayp_or_null a p)
+    (fun _ ->
+      ptr == a.from /\
+      (P.g_is_null ptr == false ==> rg == range_of_array a p)
+    )
+    (fun h _ h' -> 
+      if g_is_null a
+      then True
+      else if P.g_is_null ptr
+      then True
+      else (h' (varrayp a p) <: Seq.seq t) == (h (P.vptr_range ptr rg) <: Seq.seq t)
+    )
+
+let intro_varrayp_or_null ptr rg a p
+=
+  if g_is_null a
+  then begin
+    P.assert_null ptr _;
+    change_equal_slprop emp (varrayp_or_null a p)
+  end
+  else begin
+    P.assert_not_null ptr _;
+    intro_varrayp ptr rg a p;
+    change_equal_slprop
+      (varrayp a p)
+      (varrayp_or_null a p)
+  end
 
 let malloc x n =
-  let s = Seq.create (U32.v n) x in
-  malloc s
+  let p = P.calloc x n in
+  let res = {
+    from = p;
+    to = Ghost.hide (if P.g_is_null p then zero_size else n);
+    free_perm = full_perm;
+    prf = ();
+  } in
+  intro_varrayp_or_null p _ res full_perm;
+  return res
 
-let index r i =
-  let h = get() in
-  let s = read r in
-  Seq.index s (U32.v i)
+let indexp r p i =
+  (* TODO: we should make Steel.Pointer support indexing with size_t in addition to ptrdiff_t.
+     For now we do things manually, which will extract to ugly pointer arithmetic
+  *)
+  elim_varrayp r _;
+  let pacc = P.add r.from _ i in
+  let _ = P.move r.from pacc _ in
+  let res = P.index pacc _ zero_ptrdiff in
+  let _ = P.move pacc r.from _ in
+  intro_varrayp r.from _ r p;
+  return res
 
 let upd r i x =
-  let s = read r in
-  let s' = Seq.upd s (U32.v i) x in
-  write r s'
+  (* TODO: same here *)
+  elim_varrayp r _;
+  let pacc = P.add r.from _ i in
+  let _ = P.move r.from pacc _ in
+  P.index_upd pacc _ zero_ptrdiff x;
+  let _ = P.move pacc r.from _ in
+  intro_varrayp r.from _ r _
 
-let free r = free r
+let free r =
+  elim_varrayp r _;
+  P.free r.from _
+
+let share a p =
+  elim_varrayp a _;
+  let r = P.share a.from _ in
+  intro_varrayp a.from _ a r.P.range_write_perm;
+  intro_varrayp a.from _ a r.P.range_write_perm;
+  r.P.range_write_perm
+
+let gather a p1 p2 =
+  elim_varrayp a p1;
+  elim_varrayp a p2;
+  let r = P.gather a.from (range_of_array a p1) (range_of_array a p2) in
+  intro_varrayp a.from _ a r.P.range_write_perm;
+  r.P.range_write_perm
